Coq/Reduction.v
@@ -8,25 +8,25 @@ Require Import FunctionalExtensionality.
 
 
 Inductive Red : Contr -> Env -> ExtEnv -> Contr -> Trans -> Prop :=
-| red_zero vars rho : Red Zero vars rho Zero empty_trans
-| red_let e vars rho c c' t v :  E[| e |] vars rho = Some v -> Red c (v::vars) rho c' t ->
-               Red (Let e c) vars rho (Let (adv_exp (-1) e) c') t
-| red_transf c p1 p2 vars rho : Red (Transfer c p1 p2) vars rho Zero (singleton_trans c p1 p2 1)
-| red_scale e vars rho c c' t v :  E[| e |] vars rho = Some (RVal v) -> Red c vars rho c' t ->
-               Red (Scale e c) vars rho (Scale (adv_exp (-1) e) c') (scale_trans v t)
-| red_trans0 c vars rho c' t : Red c vars rho c' t -> Red (Translate 0 c) vars rho c' t
-| red_transS c vars rho n : Red (Translate (S n) c) vars rho (Translate n c) empty_trans
-| red_both c1 c1' c2 c2' vars rho t1 t2 : Red c1 vars rho c1' t1 -> Red c2 vars rho c2' t2 -> 
-                         Red (Both c1 c2) vars rho (Both c1' c2') (add_trans t1 t2)
-| red_if0_false vars rho c1 c2 c' b t : E[|b|] vars rho = Some (BVal false) -> 
-                                        Red c2 vars rho c' t -> Red (If b 0 c1 c2) vars rho c' t
-| red_ifS_false vars rho c1 c2 n b : E[|b|] vars rho = Some (BVal false) -> Red (If b (S n) c1 c2) vars rho (If b n c1 c2) empty_trans
-| red_if_true vars rho c1 c2 c' n b t : E[|b|] vars rho = Some (BVal true) -> Red c1 vars rho c' t -> Red (If b n c1 c2) vars rho c' t
+| red_zero env ext : Red Zero env ext Zero empty_trans
+| red_let e env ext c c' t v :  E[| e |] env ext = Some v -> Red c (v::env) ext c' t ->
+               Red (Let e c) env ext (Let (adv_exp (-1) e) c') t
+| red_transf c p1 p2 env ext : Red (Transfer c p1 p2) env ext Zero (singleton_trans c p1 p2 1)
+| red_scale e env ext c c' t v :  E[| e |] env ext = Some (RVal v) -> Red c env ext c' t ->
+               Red (Scale e c) env ext (Scale (adv_exp (-1) e) c') (scale_trans v t)
+| red_trans0 c env ext c' t : Red c env ext c' t -> Red (Translate 0 c) env ext c' t
+| red_transS c env ext n : Red (Translate (S n) c) env ext (Translate n c) empty_trans
+| red_both c1 c1' c2 c2' env ext t1 t2 : Red c1 env ext c1' t1 -> Red c2 env ext c2' t2 -> 
+                         Red (Both c1 c2) env ext (Both c1' c2') (add_trans t1 t2)
+| red_if0_false env ext c1 c2 c' b t : E[|b|] env ext = Some (BVal false) -> 
+                                        Red c2 env ext c' t -> Red (If b 0 c1 c2) env ext c' t
+| red_ifS_false env ext c1 c2 n b : E[|b|] env ext = Some (BVal false) -> Red (If b (S n) c1 c2) env ext (If b n c1 c2) empty_trans
+| red_if_true env ext c1 c2 c' n b t : E[|b|] env ext = Some (BVal true) -> Red c1 env ext c' t -> Red (If b n c1 c2) env ext c' t
 .
 
 Hint Constructors Red.
 
-Theorem red_sound1 c c' vars rho tr t  : Red c vars rho c' t ->  C[|c|] vars rho = Some tr -> tr 0 = t.
+Theorem red_sound1 c c' env ext tr t  : Red c env ext c' t ->  C[|c|] env ext = Some tr -> tr 0 = t.
 Proof.
   intro R. generalize dependent tr. induction R; simpl; intros tr T. 
   - inversion T. reflexivity.
@@ -43,8 +43,8 @@ Proof.
   - destruct n; simpl in *; rewrite H in T; auto.
 Qed.
 
-Theorem red_sound2 c c' i vars rho t t1 t2 : 
-  Red c vars rho c' t -> C[|c|]vars rho = Some t1 -> C[|c'|] vars (adv_ext 1 rho) = Some t2
+Theorem red_sound2 c c' i env ext t t1 t2 : 
+  Red c env ext c' t -> C[|c|]env ext = Some t1 -> C[|c'|] env (adv_ext 1 ext) = Some t2
   -> t1 (S i) = t2 i.
 Proof.
   intros R T1 T2. generalize dependent t1. generalize dependent t2. induction R; simpl;intros.
@@ -73,9 +73,9 @@ Qed.
 
 Ltac eauto_destruct := repeat(match goal with [ H : exists _, _ |- _] => destruct H end); eauto.
 
-Theorem red_complete c vars rho t : C[|c|] vars rho = Some t -> exists c', Red c vars rho c' (t 0).
+Theorem red_complete c env ext t : C[|c|] env ext = Some t -> exists c', Red c env ext c' (t 0).
 Proof.
-  generalize dependent t. generalize dependent vars. induction c; simpl; intros.
+  generalize dependent t. generalize dependent env. induction c; simpl; intros.
   - inversion H. eauto.
   - option_inv' H. apply IHc in H3. eauto_destruct.
   - inversion H. simpl. eauto.
@@ -87,7 +87,7 @@ Proof.
     + eauto.
   -  unfold add_trace in *. option_inv' H. apply IHc1 in H1. apply IHc2 in H2.
      eauto_destruct.
-  - remember (E[|e|]vars rho) as B. destruct B as [b'| ]. 
+  - remember (E[|e|]env ext) as B. destruct B as [b'| ]. 
     + destruct b'. destruct b.
       * destruct n; simpl in *; rewrite <- HeqB in *; apply IHc1 in H;
         eauto_destruct. 
@@ -99,58 +99,58 @@ Proof.
 Qed.
 
 
-Fixpoint RedFun (c : Contr) (vars : Env) (rho : ExtEnv) : option (Contr * Trans) :=
+Fixpoint RedFun (c : Contr) (env : Env) (ext : ExtEnv) : option (Contr * Trans) :=
   match c with
     | Zero => Some (Zero, empty_trans)
-    | Let e c => E[|e|]vars rho >>= fun val => liftM (fun res : (Contr * Trans) => 
+    | Let e c => E[|e|]env ext >>= fun val => liftM (fun res : (Contr * Trans) => 
                                                         let (c', t) := res in (Let (adv_exp (-1) e) c', t)) 
-                                                     (RedFun c (val::vars) rho)
+                                                     (RedFun c (val::env) ext)
     | Transfer c p1 p2 => Some (Zero, singleton_trans c p1 p2 1)
-    | Scale e c => match RedFun c vars rho, E[|e|]vars rho with
+    | Scale e c => match RedFun c env ext, E[|e|]env ext with
                        | Some (c', t), Some (RVal v) => Some (Scale (adv_exp (-1) e) c', scale_trans v t)
                        | _, _ => None
                    end
     | Translate l c => match l with
-                      | O => RedFun c vars rho
+                      | O => RedFun c env ext
                       | S l' => Some (Translate l' c, empty_trans)
                     end
-    | Both c1 c2 => match RedFun c1 vars rho, RedFun c2 vars rho with
+    | Both c1 c2 => match RedFun c1 env ext, RedFun c2 env ext with
                       | Some (c1', t1), Some (c2', t2) => Some (Both c1' c2', add_trans t1 t2)
                       | _, _ => None
                     end
-    | If b l c1 c2 => match E[|b|] vars rho with
+    | If b l c1 c2 => match E[|b|] env ext with
                               | Some (BVal false) => match l with
-                                                | O => RedFun c2 vars rho
+                                                | O => RedFun c2 env ext
                                                 | S l' => Some (If b l' c1 c2, empty_trans)
                                               end
-                              | Some (BVal true) => RedFun c1 vars rho
+                              | Some (BVal true) => RedFun c1 env ext
                               | _ => None
                             end
   end.
 
-Lemma redfun_red c vars rho c' t : RedFun c vars rho = Some (c', t) -> Red c vars rho c' t.
+Lemma redfun_red c env ext c' t : RedFun c env ext = Some (c', t) -> Red c env ext c' t.
 Proof.
-  generalize dependent c'. generalize dependent t. generalize dependent vars.
-  induction c; intros vars t c' R; simpl in R; try solve [inversion R;auto].
+  generalize dependent c'. generalize dependent t. generalize dependent env.
+  induction c; intros env t c' R; simpl in R; try solve [inversion R;auto].
   - option_inv_auto. destruct x0. apply IHc in H2. inversion H3.
     eauto.
-  - remember (RedFun c vars rho) as RF. destruct RF. destruct p. 
-    remember (E[|e|]vars rho) as RS. destruct RS. destruct v. inversion R.
+  - remember (RedFun c env ext) as RF. destruct RF. destruct p. 
+    remember (E[|e|]env ext) as RS. destruct RS. destruct v. inversion R.
     inversion R. auto. inversion R. inversion R.
   - destruct n. auto. inversion R. auto.
-  - specialize IHc1 with (vars:=vars). specialize IHc2 with (vars:=vars). 
-    destruct (RedFun c1 vars rho) as [p1| ]. destruct (RedFun c2 vars rho) as [p2| ].
+  - specialize IHc1 with (env:=env). specialize IHc2 with (env:=env). 
+    destruct (RedFun c1 env ext) as [p1| ]. destruct (RedFun c2 env ext) as [p2| ].
     destruct p1, p2. inversion R. auto. destruct p1. inversion R. inversion R.
-  - remember (E[|e|] vars rho) as BS. destruct BS. destruct v. destruct b. constructor; auto.
+  - remember (E[|e|] env ext) as BS. destruct BS. destruct v. destruct b. constructor; auto.
     destruct n. constructor; auto. inversion R. constructor; auto. inversion R.
     inversion R.
 Qed.
 
 
-Lemma red_redfun c vars rho c' t : Red c vars rho c' t -> RedFun c vars rho = Some (c', t).
+Lemma red_redfun c env ext c' t : Red c env ext c' t -> RedFun c env ext = Some (c', t).
 Proof.
   intros R. induction R; simpl; repeat (simpl;rewr_assumption); auto. 
 Qed.
 
-Theorem Red_function c vars rho c' t : RedFun c vars rho = Some (c', t) <-> Red c vars rho c' t.
+Theorem Red_function c env ext c' t : RedFun c env ext = Some (c', t) <-> Red c env ext c' t.
 Proof. split. apply redfun_red. apply red_redfun. Qed.
